theories/concur/relaxed.v
@@ -1,0 +1,353 @@
+From Coq Require Import Relations.
+From RelationAlgebra Require Import lattice monoid rel boolean kat_tac.
+From mathcomp Require Import ssreflect ssrbool ssrfun ssrnat seq tuple.
+From mathcomp Require Import eqtype choice order generic_quotient.
+From mathcomp Require Import fintype finfun finset fingraph finmap zify.
+From eventstruct Require Import utils rel relalg inhtype ident order.
+From eventstruct Require Import lts lposet pomset pomset_lts.
+
+Set Implicit Arguments.
+Unset Strict Implicit.
+Unset Printing Implicit Defensive.
+
+Local Open Scope order_scope.
+Local Open Scope fset_scope.
+Local Open Scope ident_scope.
+Local Open Scope lposet_scope.
+Local Open Scope pomset_scope.
+
+Module Lab.
+
+Module Lab.
+Section ClassDef.
+Record mixin_of (T0 : Type) (b : Choice.class_of T0)
+                (T := Choice.Pack b) := Mixin {
+  bot : T;
+  com : {fset T} -> T -> bool;
+  cf  : rel T;
+  is_write : pred T;
+  is_read  : pred T;
+  _ : forall w, reflect (exists ws r, com ws r /\ w \in ws) (is_write w);
+  _ : forall r, reflect (exists ws,   com ws r            ) (is_read  r);
+  _ : ~~ is_write bot;
+  _ : ~~ is_read  bot;
+}.
+
+Set Primitive Projections.
+
+Record class_of (T : Type) := Class {
+  base   : Choice.class_of T;
+  mixin  : mixin_of base;
+}.
+
+Unset Primitive Projections.
+
+Local Coercion base : class_of >-> Choice.class_of.
+
+Structure type := Pack { sort; _ : class_of sort }.
+
+Local Coercion sort : type >-> Sortclass.
+
+Variables (T : Type) (cT : type).
+
+Definition class := let: Pack _ c as cT' := cT return class_of cT' in c.
+Definition clone c of phant_id class c := @Pack T c.
+
+Definition pack :=
+  fun b bT & phant_id (Choice.class bT) b => fun m => Pack (@Class T b m).
+
+Definition eqType := @Equality.Pack cT class.
+Definition choiceType := @Choice.Pack cT class.
+End ClassDef.
+
+Module Exports.
+Coercion base : class_of >-> Choice.class_of.
+Coercion mixin : class_of >-> mixin_of.
+Coercion sort : type >-> Sortclass.
+Coercion eqType : type >-> Equality.type.
+Coercion choiceType : type >-> Choice.type.
+Canonical eqType.
+Canonical choiceType.
+Notation labType := type.
+Notation LabType T m := (@pack T _ _ id m).
+End Exports.
+
+End Lab.
+
+Export Lab.Exports.
+
+Variant typ := Read | Write | ReadWrite | Undef.
+
+Definition eq_typ : rel typ := 
+  fun t1 t2 => match t1, t2 with
+  | Read     , Read      => true
+  | Write    , Write     => true
+  | ReadWrite, ReadWrite => true
+  | Undef    , Undef     => true
+  | _ , _                => false
+  end.
+
+Lemma eq_typP : Equality.axiom eq_typ.
+Proof. by case; case; constructor. Qed.
+
+Module Export Def.
+Section Def.
+Context {L : labType}.
+Implicit Types (l : L).
+
+Definition bot : L := Lab.bot (Lab.class L).
+
+Definition com : {fset L} -> L -> bool := Lab.com (Lab.class L).
+
+Definition cf : rel L := Lab.cf (Lab.class L).
+
+Definition is_write : pred L := Lab.is_write (Lab.class L).
+Definition is_read  : pred L := Lab.is_read  (Lab.class L).
+
+Canonical typ_eqMixin := EqMixin eq_typP.
+Canonical typ_eqType  := Eval hnf in EqType typ typ_eqMixin.
+
+Definition lab_typ l : typ := 
+  if is_read l && ~~ is_write l then 
+    Read 
+  else if is_write l && ~~ is_read l then 
+    Write
+  else if is_read l && is_write l then 
+    ReadWrite
+  else Undef.
+
+End Def.
+End Def.
+
+Module Export Syntax.
+Notation "ls '|-' l"  := (com ls l) (at level 90).
+Notation "l1 '\#' l2" := (cf l1 l2) (at level 90).
+End Syntax.
+
+Module Export Theory.
+Section Theory.
+Context (L : labType).
+Implicit Types (l r w: L).
+
+Lemma is_writeP w : 
+  reflect (exists ws r, com ws r /\ w \in ws) (is_write w).
+Proof. by move: w; case L=> ? [? []]. Qed.
+
+Lemma is_readP r : 
+  reflect (exists ws, com ws r) (is_read r).
+Proof. by move: r; case L=> ? [? []]. Qed.
+
+Lemma bot_nwrite : 
+  ~~ is_write (bot : L).
+Proof. by case L=> ? [? []]. Qed.
+
+Lemma bot_nread : 
+  ~~ is_read (bot : L).
+Proof. by case L=> ? [? []]. Qed.
+
+End Theory.
+End Theory.
+
+End Lab.
+
+Export Lab.Lab.Exports.
+Export Lab.Def.
+Export Lab.Syntax.
+Export Lab.Theory.
+
+
+Module Export ThrdPomset.
+
+Notation thrd_pomset E L Tid := 
+  (@pomset E _ (\i0 : Tid, bot : L)).
+
+Notation thrd_pomlang E L Tid := 
+  (@pomset E _ (\i0 : Tid, bot : L) -> Prop).
+
+Section Def.
+Context {E : identType} {L : labType}.
+Context {Tid : identType}.
+(* data-type semantics *)
+Context (DS : ltsType L).
+(* thread semantics *)
+Context (TS : ltsType L).
+Implicit Types (d : DS) (s : TS).
+Implicit Types (p q : @thrd_pomset E L Tid).
+
+Definition fs_tid p e := 
+  fst (fs_lab p e).
+
+Definition fs_tids p := 
+  [fset (fs_tid p e) | e in finsupp p].
+
+Definition fs_dlab p e := 
+  snd (fs_lab p e).
+
+Definition fs_typ p e := 
+  lab_typ (fs_dlab p e).
+
+Definition dlab_defined p := 
+  [forall e : finsupp p, fs_dlab p (val e) != bot].
+
+Definition lab_prj : Tid * L -> L := snd.
+
+Definition lts_thrd_pomlang d : thrd_pomlang E L Tid := 
+  fun p => (lts_pomlang d : pomlang E L bot) (Pomset.relabel lab_prj p).
+
+Definition respects_com d : thrd_pomlang E L Tid := 
+  fun p => forall e, exists (es : {fset E}), 
+    [/\ (fs_dlab p) @` es |- (fs_dlab p e)
+      & forall e', e' \in es -> e' <= e :> [Event of p]
+    ].
+
+Definition cf_commute d := forall (u v : seq L) (a b : L), 
+  let Dlang := lts_lang d in
+  ~ (a \# b) -> (Dlang (u ++ [:: a ; b] ++ v) <-> Dlang (u ++ [:: b ; a] ++ v)).
+
+Lemma lab_prj_bot :
+  lab_prj (\i0, bot) = bot.
+Proof. done. Qed.
+
+End Def.
+
+End ThrdPomset.
+
+Section ProgramOrder.
+Context {E : identType} {L : labType}.
+Context {Tid : identType}.
+(* thread semantics *)
+Context (TS : ltsType L).
+Implicit Types (p q : @thrd_pomset E L Tid).
+
+Definition eq_tid p : rel E := 
+  fun e1 e2 => fs_tid p e1 == fs_tid p e2.
+
+Arguments eq_tid p : clear implicits. 
+
+Lemma eqtid_refl p : reflexive (eq_tid p).
+Proof. by rewrite /eq_tid. Qed.
+
+Lemma eqtid_sym p : symmetric (eq_tid p).
+Proof. by rewrite /eq_tid. Qed.
+
+Lemma eqtid_trans p : transitive (eq_tid p).
+Proof. by rewrite /eq_tid=> ??? /eqP-> /eqP->. Qed.
+
+Definition po p : thrd_pomset E L Tid := 
+  Pomset.inter_rel (eq_tid p) (@eqtid_refl p) (@eqtid_trans p) p.
+
+Definition po_spec p := 
+  {in (fs_tids p), forall t, exists (s0 : TS),
+    let es := [fset e | e in finsupp p & (fs_tid p e == t)] in
+    let pt := Pomset.restrict (mem es) p in
+    (lts_pomlang s0 : pomlang E L bot) (Pomset.relabel lab_prj pt)
+  }.
+
+End ProgramOrder.
+
+
+Section SeqCst.
+Context {E : identType} {L : labType}.
+Context {Tid : identType}.
+(* data-type semantics *)
+Context (DS : ltsType L).
+(* thread semantics *)
+Context (TS : ltsType L).
+
+Implicit Types (d : DS) (s : TS).
+Implicit Types (p q : @thrd_pomset E L Tid).
+
+Definition seq_cst d p := 
+  eq (po p) \supports (lts_thrd_pomlang d).
+
+End SeqCst.
+
+(* TODO: better name? *)
+Section ValueRelab. 
+Context {E : identType} {L : labType}.
+Context {Tid : identType}.
+(* data-type semantics *)
+Context (DS : ltsType L).
+(* thread semantics *)
+Context (TS : ltsType L).
+Implicit Types (p : @thrd_pomset E L Tid).
+
+(* checks that f is a value-relabeling of pomset p w.r.t. set of events es *)
+Definition relab_mod p (es : {fset E}) (f : Tid * L -> L) := 
+  let lab e  := fs_lab  p (val e) in
+  let dlab e := fs_dlab p (val e) in
+  [&& (* types of all events are preserved (i.e. reads/writes are preserved) *)
+      [forall e : finsupp p, lab_typ (f (lab e)) == lab_typ (dlab e)]
+    , (* conflict relation is preserved *)
+      [forall e1 : finsupp p, forall e2 : finsupp p, 
+        (f (lab e1) \# f (lab e2)) == ((dlab e1) \# (dlab e2)) 
+      ]
+    & (* labels of all events not in es are preserved *)
+      [forall e : finsupp p, (val e \notin es) ==> (f (lab e) == dlab e)]
+  ].
+
+End ValueRelab. 
+
+
+Section CausalCst. 
+Context {E : identType} {L : labType}.
+Context {Tid : identType}.
+(* data-type semantics *)
+Context (DS : ltsType L).
+(* thread semantics *)
+Context (TS : ltsType L).
+
+Implicit Types (d : DS) (s : TS).
+Implicit Types (p : @thrd_pomset E L Tid).
+
+(* Causally relabeled threaded pomset language of data-structure DS.
+ * Pomset p belongs to this language if 
+ * for every event e of p, the restriction of p onto prefix of e
+ * is equiavelnt to relabeling of some q \in (lang DS) such that this relabeling
+ *   (1) preserves labels of all events from the thread of e 
+ *       and all writes events (i.e. non-reads);
+ *   (2) preserves types (i.e. reads/writes) of all events.
+ *)
+Definition causal d p := 
+  {in (finsupp p), forall e, exists f,
+    let rst := pideal (e : [Event of p]) in
+    let ro := 
+      [fset e' in finsupp p | (fs_typ p e' == Lab.Read) && ~~ (eq_tid p e e')]
+    in
+    let p_rlb := Pomset.relabel f p in  
+    let p_rst := Pomset.restrict (mem rst) p_rlb in
+    [/\ relab_mod p ro f
+      & eq (p_rst) \supports (lts_pomlang d : pomlang E L bot)
+    ]
+  }.
+  
+Definition causal_cst d p := 
+  eq (po p) \supports (causal d).  
+
+
+End CausalCst.
+
+
+Section PipeCst. 
+Context {E : identType} {L : labType}.
+Context {Tid : identType}.
+(* data-type semantics *)
+Context (DS : ltsType L).
+(* thread semantics *)
+Context (TS : ltsType L).
+
+Implicit Types (d : DS) (s : TS).
+Implicit Types (p : @thrd_pomset E L Tid).
+
+Definition pipe_cst d p := 
+  {in (fs_tids p), forall t, exists f,
+    let prv := 
+      [fset e' in finsupp p | (fs_tid p e' == t) || ~~ is_read (fs_dlab p e')]
+    in
+    let po_rlb := Pomset.relabel f (po p) in  
+    [/\ relab_mod p prv f
+      & eq po_rlb \supports (lts_pomlang d : pomlang E L bot)
+    ]
+  }.
+
+End PipeCst.
